run_all_experiments.sh
@@ -1,0 +1,16 @@
+#! /bin/bash
+
+for f in ./blocks/*.txt;  do
+    nlines=`wc -l < $f`
+    nblocks=$(( nlines/3 ))
+	echo "$f"
+	echo "($nblocks blocks)";
+	echo '---------------------------------'
+	n0=`./bin/checker -alg 0 < $f | grep true | wc -l`
+	n1=`./bin/checker -alg 1 < $f | grep true | wc -l`
+	n2=`./bin/checker -alg 2 < $f | grep true | wc -l`
+	echo "* evm_eq_block_chkr (CHKR): $n0"
+    echo "* evm_eq_block_chkr' (CHKR') : $n1"
+    echo "* evm_eq_block_chkr'' (CHKR'') : $n2"
+	echo
+done;
